coq_translation/examples-from-rust-book/generics/generics_associated_types_problem.v
@@ -4,13 +4,13 @@ Require Import CoqOfRust.CoqOfRust.
 Import Root.std.prelude.rust_2015.
 
 Module Container.
-  Inductive t : Set := Build (_ : i32) (_ : i32).
+  Record t : Set := { _ : i32; _ : i32;}.
   
-  Global Instance Get_0 : IndexedField.Class t 0 _ := {
-    IndexedField.get '(Build x0 _) := x0;
+  Global Instance Get_0 : Notation.Dot 0 := {
+    Notation.dot '(Build_t x0 _) := x0;
   }.
-  Global Instance Get_1 : IndexedField.Class t 1 _ := {
-    IndexedField.get '(Build _ x1) := x1;
+  Global Instance Get_1 : Notation.Dot 1 := {
+    Notation.dot '(Build_t _ x1) := x1;
   }.
 End Container.
 Definition Container := Container.t.
